#+LATEX_HEADER: \newcommand{\Incr}{{+}\hspace{-4pt}{+}}

* Exercises 2.2
** 2.2.1 Prove Proposition 2.2.5 (Hint: fix two of the variables and induct on the third)

*Proposition 2.2.5* /(Addition is associative)/

/For any natural numbers $a,b,c$, 
we have $(a+b)+c=a+(b+c)$./

$-------------------------------------------------------------------------$

$\bullet~~$ Show that $(a+b)+c=a+(b+c)$ for each $a,b,c\in\mathbb{N}$.

$\Vdash~~$ {Proof by induction on $a$}

$\hspace{16pt}\bullet~~$ Base case: show that $(a+b)+c=a+(b+c)$, when
  
$\hspace{16pt}--~~$ $a=0$
 
$\hspace{16pt}\Vdash~~$ $(a+b)+c=a+(b+c)$
 
$\hspace{16pt}\equiv~~$ {substitute assumption $a=0$}

$\hspace{32pt}$ $(0+b)+c=0+(b+c)$

$\hspace{16pt}\equiv~~$ {Definition 2.2.1}

$\hspace{32pt}$ $(b)+c=(b+c)$

$\hspace{16pt}\equiv~~$ {simplify}

$\hspace{32pt}$ $b+c=b+c$

$\hspace{16pt} \square$

$\hspace{16pt}\bullet~~$ Inductive step: show that $((a+\hspace{-4pt}+)+b)+c=(a+\hspace{-4pt}+)+(b+c)$, when

$\hspace{16pt}--~~$ $(a+b)+c=a+(b+c)$

$\hspace{16pt}\Vdash~~$ $((a+\hspace{-4pt}+)+b)+c$

$\hspace{16pt}=~~$ {Definition 2.2.1}

$\hspace{32pt}$ $((a+b)+\hspace{-4pt}+)+c$

$\hspace{16pt}=~~$ {Definition 2.2.1}

$\hspace{32pt}$ $((a+b)+c)+\hspace{-4pt}+$

$\hspace{16pt}=~~$ {inductive hypothesis}

$\hspace{32pt}$ $(a+(b+c))+\hspace{-4pt}+$

$\hspace{16pt}=~~$ {Definition 2.2.1}

$\hspace{32pt}$ $(a+\hspace{-4pt}+)+(b+c)$

$\hspace{16pt}\square$

$\square$

** 2.2.2 Prove Lemma 2.2.10. 
(Hint: use induction. the induction here is somewhat degenerate, in that the induction hypothesis is not actually used, but this does not prevent the argument from remaining valid; cf. the discussion on implication and causality in Appendix A.2.)

*Lemma 2.2.10.* 

/Let $a$ be a positive number. Then there exists exactly one natural number $b$ such that $b\hspace{-2pt}+\hspace{-4pt}+=a$./

$-------------------------------------------------------------------------$

$\bullet~~$ Show that $\forall a\in\mathbb{N}:a\neq0\implies \exists!b\in\mathbb{N}:b\hspace{-2pt}+\hspace{-4pt}+=a$.

$\Vdash~~$ {Proof by induction on $a$}

$\hspace{16pt}\bullet~~$ Base case: show that $\forall a\in\mathbb{N}:a\neq0\implies \exists!b\in\mathbb{N}:b\hspace{-2pt}+\hspace{-4pt}+=a$, when
  
$\hspace{16pt}--~~$ $a=0$

$\hspace{16pt}\Vdash~~$ $\forall a\in\mathbb{N}:a\neq0\implies \exists!b\in\mathbb{N}:b\hspace{-2pt}+\hspace{-4pt}+=a$
 
$\hspace{16pt}\equiv~~$ {substitute assumption $a=0$, implication is vacuously true since $0\neq0$ is false}

$\hspace{32pt}$ T

$\hspace{16pt}\square$

$\hspace{16pt}\bullet~~$ Inductive step: show that $\forall a\hspace{-2pt}+\hspace{-4pt}+\in\mathbb{N}:a\hspace{-2pt}+\hspace{-4pt}+\neq0\implies \exists!b\in\mathbb{N}:b\hspace{-2pt}+\hspace{-4pt}+=a\hspace{-2pt}+\hspace{-4pt}+$, when

$\hspace{16pt}--~~$ $\forall a\in\mathbb{N}:a\neq0\implies \exists!b\in\mathbb{N}:b\hspace{-2pt}+\hspace{-4pt}+=a$
  
$\hspace{16pt}\Vdash~~$ $\forall a\hspace{-2pt}+\hspace{-4pt}+\in\mathbb{N}:a\hspace{-2pt}+\hspace{-4pt}+\neq0\implies \exists!b\in\mathbb{N}:b\hspace{-2pt}+\hspace{-4pt}+=a\hspace{-2pt}+\hspace{-4pt}+$

$\hspace{32pt}\bullet~~$ Existance of $b$

$\hspace{32pt}\Vdash~~$ $\forall a\hspace{-2pt}+\hspace{-4pt}+\in\mathbb{N}:a\hspace{-2pt}+\hspace{-4pt}+\neq0\implies \exists b\in\mathbb{N}:b\hspace{-2pt}+\hspace{-4pt}+=a\hspace{-2pt}+\hspace{-4pt}+$

$\hspace{32pt}\equiv~~$ {Let $b:=a$}

$\hspace{50pt}$ $\forall a\hspace{-2pt}+\hspace{-4pt}+\in\mathbb{N}:a\hspace{-2pt}+\hspace{-4pt}+\neq0\implies a\hspace{-2pt}+\hspace{-4pt}+=a\hspace{-2pt}+\hspace{-4pt}+$

$\hspace{32pt}\equiv~~$ {Reflexive axiom}

$\hspace{50pt}$ T

$\hspace{32pt}\square$

$\hspace{32pt}\bullet~~$ Uniqueness of $b$

$\hspace{32pt}\Vdash~~$ $\forall a\hspace{-2pt}+\hspace{-4pt}+\in\mathbb{N}:a\hspace{-2pt}+\hspace{-4pt}+\neq0, ~~b,c\in\mathbb{N}:b\hspace{-2pt}+\hspace{-4pt}+=a\hspace{-2pt}+\hspace{-4pt}+\land c\hspace{-2pt}+\hspace{-4pt}+=a\hspace{-2pt}+\hspace{-4pt}+\implies b=c$

$\hspace{32pt}\equiv~$ { $b=a$, $c=a$ by Axiom 2.4, then $b=a$, $a=c$ by Symmetry axiom, then $b=c$ by Transitive axiom}

$\hspace{50pt}$ T

$\hspace{32pt}\square$

$\hspace{16pt}\cdots~~$ {Since $P(n\hspace{-2pt}+\hspace{-4pt}+)$ is true, $P(n)\implies P(n\hspace{-2pt}+\hspace{-4pt}+)$ is always true whether or not $P(n)$ is true}

$\hspace{32pt}$ T

$\hspace{16pt}\square$

$\square$
